src/Init/Grind/Ordered/Linarith.lean
@@ -469,10 +469,17 @@ theorem eq_neg {α} [IntModule α] (ctx : Context α) (p₁ p₂ : Poly)
 def eq_coeff_cert (p₁ p₂ : Poly) (k : Nat) :=
   k != 0 && p₁ == p₂.mul k
 
+theorem no_nat_zero_divisors' [IntModule α] [NoNatZeroDivisors α] (k : Nat) (a : α)
+    : k ≠ 0 → k * a = 0 → a = 0 := by
+  intro h₁ h₂
+  have : k * a = (↑k : Int) * (0 : α) → a = 0 := no_nat_zero_divisors k a 0 h₁
+  rw [IntModule.hmul_zero] at this
+  exact this h₂
+
 theorem eq_coeff {α} [IntModule α] [NoNatZeroDivisors α] (ctx : Context α) (p₁ p₂ : Poly) (k : Nat)
     : eq_coeff_cert p₁ p₂ k → p₁.denote' ctx = 0 → p₂.denote' ctx = 0 := by
   simp [eq_coeff_cert]; intro h _; subst p₁; simp [*]
-  exact no_nat_zero_divisors k (p₂.denote ctx) h
+  exact no_nat_zero_divisors' k (p₂.denote ctx) h
 
 def coeff_cert (p₁ p₂ : Poly) (k : Nat) :=
   k > 0 && p₁ == p₂.mul k
@@ -517,7 +524,7 @@ theorem eq_diseq_subst {α} [IntModule α] [NoNatZeroDivisors α] (ctx : Context
       next h => rw [← h]; assumption
       next h => replace h := congrArg (- ·) h; simp at h; rw [← h, IntModule.neg_hmul, h₃, IntModule.neg_zero]
     exact this
-  have := no_nat_zero_divisors (k₁.natAbs) (p₂.denote ctx) hne this
+  have := no_nat_zero_divisors' (k₁.natAbs) (p₂.denote ctx) hne this
   contradiction
 
 def eq_diseq_subst1_cert (k : Int) (p₁ p₂ p₃ : Poly) : Bool :=
